matching-logic/src/Theories/Nat_Syntax.v
@@ -1,0 +1,94 @@
+From Coq Require Import ssreflect ssrfun ssrbool.
+
+From Ltac2 Require Import Ltac2.
+
+From Coq Require Import String Ensembles Setoid.
+Require Import Coq.Program.Equality.
+Require Import Coq.Logic.Classical_Prop.
+From Coq.Logic Require Import FunctionalExtensionality Eqdep_dec.
+From Coq.Classes Require Import Morphisms_Prop.
+From Coq.Unicode Require Import Utf8.
+From Coq.micromega Require Import Lia.
+
+From MatchingLogic Require Import Logic ProofMode.
+From MatchingLogic.Theories Require Import Definedness_Syntax Definedness_ProofSystem.
+From MatchingLogic.Utils Require Import stdpp_ext.
+
+Require Import MatchingLogic.wftactics.
+
+From stdpp Require Import base fin_sets sets propset proof_irrel option list.
+
+Import extralibrary.
+
+Import MatchingLogic.Logic.Notations.
+Import MatchingLogic.Theories.Definedness_Syntax.Notations.
+
+Set Default Proof Mode "Classic".
+
+From MatchingLogic Require Import
+  Theories.DeductionTheorem
+  Theories.Sorts_Syntax
+  FOEquality_ProofSystem
+  Sorts_ProofSystem
+.
+
+Import MatchingLogic.Theories.Sorts_Syntax.Notations.
+
+Open Scope ml_scope.
+Open Scope string_scope.
+Open Scope list_scope.
+
+
+Section nat_syntax.
+
+  Context {Σ : Signature}.
+
+  Inductive Symbols := sNat | sZero | sSucc.
+
+  Class Syntax :=
+    { inj : Symbols -> symbols;
+      imported_sorts :> Sorts_Syntax.Syntax;
+    }.
+  Context {self : Syntax}.
+
+  Definition Nat := patt_sym (inj sNat).
+  Definition Zero := patt_sym (inj sZero).
+  Definition Succ := patt_sym (inj sSucc).
+
+End nat_syntax.
+
+
+Section nat.
+  Context
+    {Σ : Signature}
+    {syntax : Syntax}
+  .
+
+  Inductive AxiomName := 
+  | AxFun1
+  | AxFun2
+  | AxNoConfusion1
+  | AxNoConfusion2
+  | AxInductiveDomain.
+
+  Definition axiom (name : AxiomName) : Pattern :=
+    match name with
+    | AxFun1 => ex Nat , Zero =ml b0
+    | AxFun2 => all Nat, ex Nat, Succ $ b1 =ml b0
+    | AxNoConfusion1 => all Nat, !(Zero =ml Succ $ b0)
+    | AxNoConfusion2 => all Nat, all Nat, (Succ $ b1 =ml Succ $ b0 ---> b1 =ml b0)
+    | AxInductiveDomain => 〚 Nat 〛 =ml mu , Zero or Succ $ B0
+    end.
+
+  Program Definition named_axioms : NamedAxioms :=
+    {|
+      NAName := AxiomName;
+      NAAxiom := axiom;
+    |}.
+  Next Obligation.
+    destruct name; simpl; wf_auto2.
+  Qed.
+
+  Definition theory := Definedness_Syntax.theory ∪ theory_of_NamedAxioms named_axioms.
+
+End nat.
